prove store_felem for curve25519.field64

code/experimental/curve25519/Hacl.Impl.Curve25519.Field64.fst
@@ -11,17 +11,28 @@ open Lib.Buffer
 include Hacl.Impl.Curve25519.Field64.Core
 
 module ST = FStar.HyperStack.ST
-module S = Hacl.Spec.Curve25519.Field64.Definition
-module Lemmas = Hacl.Spec.Curve25519.Field64.Lemmas
 module LSeq = Lib.Sequence
 module BSeq = Lib.ByteSequence
-module P = Spec.Curve25519
 
-#reset-options "--z3rlimit 20"
+module P = Spec.Curve25519
+module S = Hacl.Spec.Curve25519.Field64.Definition
+module Lemmas = Hacl.Spec.Curve25519.Field64.Lemmas
+module SC = Hacl.Spec.Curve25519.Field64
+
+#reset-options "--z3rlimit 50"
 
 let felem = lbuffer uint64 4ul
 let felem2 = lbuffer uint64 8ul
 let felem_wide = lbuffer uint64 8ul
+
+noextract
+let as_tup4 (h:mem) (f:felem) : GTot S.felem4 =
+  let s = as_seq h f in
+  let s0 = s.[0] in
+  let s1 = s.[1] in
+  let s2 = s.[2] in
+  let s3 = s.[3] in
+  (s0, s1, s2, s3)
 
 inline_for_extraction
 val create_felem:
@@ -51,6 +62,20 @@ let load_felem f u64s =
   f.(3ul) <- u64s.(3ul)
 
 inline_for_extraction
+val carry_pass_store:
+    f:felem
+ -> Stack unit
+   (requires fun h -> live h f)
+   (ensures fun h0 _ h1 ->
+     modifies (loc f) h0 h1 /\
+     as_nat h1 f == S.as_nat4 (SC.carry_pass_store (as_tup4 h0 f)))
+let carry_pass_store f =
+  let f3 = f.(3ul) in
+  let top_bit = f3 >>. 63ul in
+  f.(3ul) <- f3 &. u64 0x7fffffffffffffff;
+  let carry = add1 f f (u64 19 *! top_bit) in ()
+
+inline_for_extraction
 val store_felem:
     u64s:lbuffer uint64 4ul
   -> f:felem
@@ -58,23 +83,31 @@ val store_felem:
     (requires fun h ->
       live h f /\ live h u64s /\ disjoint u64s f)
     (ensures  fun h0 _ h1 ->
-      modifies (loc u64s |+| loc f) h0 h1)
-     // BSeq.nat_from_intseq_le (as_seq h1 u64s) == (as_nat h0 f) % P.prime)
+      modifies (loc u64s |+| loc f) h0 h1 /\
+      BSeq.nat_from_intseq_le (as_seq h1 u64s) == (as_nat h0 f) % P.prime)
 let store_felem u64s f =
+  let h0 = ST.get () in
+  carry_pass_store f;
+  let h1 = ST.get () in
+  SC.lemma_carry_pass_store0 (as_tup4 h0 f);
+  carry_pass_store f;
+  let h2 = ST.get () in
+  SC.lemma_carry_pass_store1 (as_tup4 h1 f);
+  let f0 = f.(0ul) in
+  let f1 = f.(1ul) in
+  let f2 = f.(2ul) in
   let f3 = f.(3ul) in
-  let top_bit = f3 >>. 63ul in
-  f.(3ul) <- f3 &. u64 0x7fffffffffffffff;
-  let carry = add1 f f (u64 19 *. top_bit) in
-
-  let f3 = f.(3ul) in
-  let top_bit = f3 >>. 63ul in
-  f.(3ul) <- f3 &. u64 0x7fffffffffffffff;
-  let carry = add1 f f (u64 19 *. top_bit) in
-
-  u64s.(0ul) <- f.(0ul);
-  u64s.(1ul) <- f.(1ul);
-  u64s.(2ul) <- f.(2ul);
-  u64s.(3ul) <- f.(3ul)
+  assert (v f3 < pow2 63);
+  assert (as_nat h2 f < pow2 255);
+  let (o0, o1, o2, o3) = SC.subtract_p4 (f0, f1, f2, f3) in
+  assert (S.as_nat4 (o0, o1, o2, o3) < P.prime);
+  assert (S.as_nat4 (o0, o1, o2, o3) == (as_nat h2 f) % P.prime);
+  u64s.(0ul) <- o0;
+  u64s.(1ul) <- o1;
+  u64s.(2ul) <- o2;
+  u64s.(3ul) <- o3;
+  let h3 = ST.get () in
+  Lemmas.lemma_nat_from_uints64_le_4 (as_seq h3 u64s)
 
 inline_for_extraction
 val set_zero:
