code/experimental/curve25519/Hacl.Helpers.fst
@@ -1,0 +1,78 @@
+module Hacl.Helpers
+
+open Lib.IntTypes
+
+let uint64_eq_mask (a:uint64) (b:uint64) : uint64 =
+  let x = a ^. b in
+  let minus_x = (lognot x) +. (u64 1) in
+  let x_or_minus_x = x |. minus_x in
+  let xnx = x_or_minus_x >>. 63ul in
+  let c = xnx -. (u64 1) in
+  c
+
+let uint64_gte_mask (a:uint64) (b:uint64) : uint64 =
+  let x = a in
+  let y = b in
+  let x_xor_y = logxor x y in
+  let x_sub_y = x -. y in
+  let x_sub_y_xor_y = x_sub_y ^. y in
+  let q = logor x_xor_y x_sub_y_xor_y in
+  let x_xor_q = logxor x q in
+  let x_xor_q_ = shift_right x_xor_q 63ul in
+  let c = sub_mod x_xor_q_ (u64 1) in
+  c
+
+val uint64_eq_mask_logand_lemma: a:uint64 -> b:uint64 -> c:uint64 ->
+  Lemma
+  (requires True)
+  (ensures
+    (if v a = v b then
+      v (c `logand` (uint64_eq_mask a b)) == v c
+    else
+      v (c `logand` (uint64_eq_mask a b)) == 0))
+  [SMTPat (c `logand` (uint64_eq_mask a b))]
+let uint64_eq_mask_logand_lemma a b c = admit()
+
+val uint64_gte_mask_logand_lemma: a:uint64 -> b:uint64 -> c:uint64 ->
+  Lemma
+  (requires True)
+  (ensures
+    (if v a >= v b then
+      v (c `logand` (uint64_gte_mask a b)) == v c
+    else
+      v (c `logand` (uint64_gte_mask a b)) == 0))
+  [SMTPat (c `logand` (uint64_gte_mask a b))]
+let uint64_gte_mask_logand_lemma a b c = admit()
+
+val uint64_eq_mask_lemma: a:uint64 -> b:uint64 ->
+  Lemma
+  (requires True)
+  (ensures
+  (if v a = v b then
+    v (uint64_eq_mask a b) == pow2 64 - 1
+  else
+    v (uint64_eq_mask a b) == 0))
+  [SMTPat (uint64_eq_mask a b)]
+let uint64_eq_mask_lemma a b = admit()
+
+val uint64_gte_mask_lemma: a:uint64 -> b:uint64 ->
+  Lemma
+  (requires True)
+  (ensures
+    (if v a >= v b then
+      v (uint64_gte_mask a b) == pow2 64 - 1
+    else
+      v (uint64_gte_mask a b) == 0))
+  [SMTPat (uint64_gte_mask a b)]
+let uint64_gte_mask_lemma a b = admit()
+
+val logand_lemma: a:uint64 -> b:uint64 ->
+  Lemma
+  (requires v a = 0 \/ v a = pow2 64 - 1)
+  (ensures
+    (if v a = 0 then
+      v (a `logand` b) == 0
+    else
+      v (a `logand` b) == v b))
+  [SMTPat (a `logand` b)]
+let logand_lemma a b = admit()
